update CLI for solinas reduction

src/PushButtonSynthesis/SolinasReduction.v
@@ -31,7 +31,8 @@ Require Import Crypto.BoundsPipeline.
 Require Import Crypto.COperationSpecifications.
 Require Import Crypto.PushButtonSynthesis.ReificationCache.
 Require Import Crypto.PushButtonSynthesis.Primitives.
-(* Require Import Crypto.PushButtonSynthesis.SaturatedSolinasReificationCache. *)
+Require Import Crypto.PushButtonSynthesis.SaturatedSolinasReificationCache.
+Require Import Crypto.PushButtonSynthesis.SolinasReductionReificationCache.
 Require Import Crypto.Assembly.Equivalence.
 Import ListNotations.
 Local Open Scope string_scope. Local Open Scope Z_scope. Local Open Scope list_scope. Local Open Scope bool_scope.
@@ -48,6 +49,7 @@ Import COperationSpecifications.Solinas.
 Import COperationSpecifications.SolinasReduction.
 
 Import Associational Positional.
+Import SolinasReduction.
 
 Local Coercion Z.of_nat : nat >-> Z.
 Local Coercion QArith_base.inject_Z : Z >-> Q.
@@ -55,7 +57,7 @@ Local Coercion Z.pos : positive >-> Z.
 
 Local Set Keyed Unification. (* needed for making [autorewrite] fast, c.f. COQBUG(https://github.com/coq/coq/issues/9283) *)
 
-Local Opaque reified_mul_gen. (* needed for making [autorewrite] not take a very long time *)
+Local Opaque reified_solmul_gen. (* needed for making [autorewrite] not take a very long time *)
 (* needed for making [autorewrite] with [Set Keyed Unification] fast *)
 Local Opaque expr.Interp.
 
@@ -86,8 +88,8 @@ Section __.
           {assembly_conventions : assembly_conventions_opt}
           {error_on_unused_assembly_functions : error_on_unused_assembly_functions_opt}
           (s : Z)
-          (c : list (Z * Z))
-          (machine_wordsize : machine_wordsize_opt).
+          (c : list (Z * Z)).
+  Context (machine_wordsize := 64).
 
   Local Existing Instance widen_bytes.
 
@@ -98,19 +100,10 @@ Section __.
 
   Definition n : nat := Z.to_nat (Qceiling (Z.log2_up s / machine_wordsize)).
   Definition m := s - Associational.eval c.
-  (* Number of reductions is calculated as follows :
-         Let i be the highest limb index of c. Then, each reduction
-         decreases the number of extra limbs by (n-i-1). (The -1 comes
-         from possibly having an extra high partial product at the end
-         of a reduction.) So, to go from the n extra limbs we have
-         post-multiplication down to 0, we need ceil (n / (n - i - 1))
-         reductions.  In some cases. however, [n - i <= 1], and in
-         this case, we do [n] reductions (is this enough?). *)
-  Definition nreductions : nat :=
-    let i := fold_right Z.max 0 (List.map (fun t => Z.log2 (fst t) / machine_wordsize) c) in
-    if Z.of_nat n - i <=? 1
-    then n
-    else Z.to_nat (Qceiling (Z.of_nat n / (Z.of_nat n - i - 1))).
+  Definition weight := UniformWeight.uweight machine_wordsize.
+  Definition up_bound := 2 ^ (machine_wordsize / 4).
+  Definition base := 2 ^ machine_wordsize.
+
   Let possible_values := possible_values_of_machine_wordsize.
   Definition bound := Some r[0 ~> (2^machine_wordsize - 1)]%zrange.
   Definition boundsn : list (ZRange.type.option.interp base.type.Z)
@@ -127,13 +120,19 @@ Section __.
     := check_args_of_list
          (List.map
             (fun v => (true, v))
-            [((0 <? s - Associational.eval c)%Z, Pipeline.Value_not_ltZ "s - Associational.eval c ≤ 0" 0 (s - Associational.eval c))
+            [((0 <? s)%Z, Pipeline.Value_not_ltZ "0 < s" 0 s)
+             ; ((0 <? Associational.eval c)%Z, Pipeline.Value_not_ltZ "0 < Associational.eval c" 0 (Associational.eval c))
+             ; ((0 <? s - Associational.eval c)%Z, Pipeline.Value_not_ltZ "s - Associational.eval c ≤ 0" 0 (s - Associational.eval c))
              ; (negb (s =? 0)%Z, Pipeline.Values_not_provably_distinctZ "s ≠ 0" s 0)
              ; (negb (n =? 0)%nat, Pipeline.Values_not_provably_distinctZ "n ≠ 0" n 0)
              ; (0 <? machine_wordsize, Pipeline.Value_not_ltZ "0 < machine_wordsize" 0 machine_wordsize)
+             ; ((1 <? n)%nat, Pipeline.Value_not_ltZ "1 < n" 1 n)
+             ; (fst (Rows.adjust_s weight (S (S n)) s) =? weight n, Pipeline.Values_not_provably_equalZ "fst (Rows.adjust_s weight (S (S n)) s) = weight n" (fst (Rows.adjust_s weight (S (S n)) s)) (weight n))
+             ; (snd (Rows.adjust_s weight (S (S n)) s), Pipeline.Invalid_argument "tmp")
+             ; (weight n / s * Associational.eval c <? up_bound, Pipeline.Value_not_ltZ "weight n / s * Associational.eval c < up_bound" (weight n / s * Associational.eval c) up_bound)
          ])
          res.
-
+Locate ErrorMessage.
 
   Local Ltac use_curve_good_t :=
     repeat first [ use_requests_to_prove_curve_good_t_step
@@ -146,23 +145,35 @@ Section __.
           (curve_good : check_args requests (Success tt) = Success tt).
 
   Lemma use_curve_good
-    : 0 < s - Associational.eval c
-      /\ s - Associational.eval c <> 0
-      /\ s <> 0
-      /\ 0 < machine_wordsize
-      /\ n <> 0%nat.
+    : (n > 1)%nat /\
+        s > 0 /\
+        Associational.eval c > 0 /\
+        s - Associational.eval c <> 0 /\
+        base <> 0 /\
+        Rows.adjust_s weight (S (S n)) s = (weight n, true) /\
+        weight n / s * Associational.eval c < up_bound.
   Proof using curve_good.
     prepare_use_curve_good ().
     { use_curve_good_t. }
+    { use_curve_good_t. }
+    { unfold base.
+      use_curve_good_t. }
+    { lazymatch goal with
+      | |- ?x = _ => rewrite surjective_pairing with (p:=x)
+      end.
+      repeat match goal with
+             | H : ?x = _ |- (?x, _) = _ => rewrite H
+             | H : ?x = _ |- (_, ?x) = _ => rewrite H
+             end.
+      auto. }
   Qed.
 
-  Local Notation weightf := (weight machine_wordsize 1).
-  Local Notation evalf := (eval weightf n).
+  Local Notation evalf := (eval weight n).
   Local Notation notations_for_docstring
     := (CorrectnessStringification.dyn_context.cons
-          weightf "weight"
+          evalf "eval"
           (CorrectnessStringification.dyn_context.cons
-             evalf "eval"
+             weight "weight"
              CorrectnessStringification.dyn_context.nil))%string.
   Local Notation "'docstring_with_summary_from_lemma!' summary correctness"
     := (docstring_with_summary_from_lemma_with_ctx!
@@ -176,10 +187,13 @@ Section __.
          false (* subst01 *)
          None (* fancy *)
          possible_values
-         (reified_mul_gen
-            @ GallinaReify.Reify s @ GallinaReify.Reify c @ GallinaReify.Reify (machine_wordsize:Z) @ GallinaReify.Reify n @ GallinaReify.Reify nreductions)
+         (reified_solmul_gen
+            @GallinaReify.Reify base
+            @GallinaReify.Reify s
+            @GallinaReify.Reify c
+            @GallinaReify.Reify n )
          (Some boundsn, (Some boundsn, tt))
-         (Some boundsn, None (* Should be: Some r[0~>0]%zrange, but bounds analysis is not good enough *) ).
+         (Some boundsn).
 
   Definition smul (prefix : string)
     : string * (Pipeline.ErrorT (Pipeline.ExtendedSynthesisResult _))
@@ -188,21 +202,20 @@ Section __.
           machine_wordsize prefix "mul" mul
           (docstring_with_summary_from_lemma!
              (fun fname : string => [text_before_function_name ++ fname ++ " multiplies two field elements."]%string)
-             (mul_correct weightf n m boundsn)).
+             (mulmod_correct weight n m boundsn)).
 
   Local Ltac solve_extra_bounds_side_conditions :=
     cbn [lower upper fst snd] in *; Bool.split_andb; Z.ltb_to_lt; lia.
 
   Hint Rewrite
-       (fun pf => @Rows.eval_mulmod (weight machine_wordsize 1) (@wprops _ _ pf))
-       using solve [ auto with zarith | congruence | solve_extra_bounds_side_conditions ] : push_eval.
+       (fun pf => @SolinasReduction.SolinasReduction.mulmod_correct (@wprops _ _ pf)) using solve [ auto with zarith | congruence | solve_extra_bounds_side_conditions ] : push_eval.
   Hint Unfold mulmod : push_eval.
 
   Local Ltac prove_correctness _ := Primitives.prove_correctness use_curve_good.
 
   Lemma mul_correct res
         (Hres : mul = Success res)
-    : mul_correct (weight machine_wordsize 1) n m boundsn (Interp res).
+    : mulmod_correct weight n m boundsn (Interp res).
   Proof using curve_good. prove_correctness (). Qed.
 
   Lemma Wf_mul res (Hres : mul = Success res) : Wf res.
@@ -228,8 +241,7 @@ Section __.
                (comment_header
                   ++ ["";
                      "Computed values:";
-                     "";
-                     "  # reductions = " ++ show nreductions]%string)))
+                     ""]%string)))
            function_name_prefix requests.
   End for_stringification.
 End __.
